# 2018-3

在 $X = C[0, 1]$ 上赋予范数 $\|x\|_1 = \int_0^1 |x(t)| dt$。若 $x \in X$，令

$$
\begin{aligned}
f_1(x) &= x(0)\\
f_2(x) &= \int_0^1 tx(t) dt\\
\end{aligned}
$$

求证：

1. $f_1, f_2$ 都是 $X$ 上的线性泛函
2. $f_1 \notin X'$
3. $f_2 \in X'$，求出 $\|f_2\|$

## 解答

### 1. $f_1, f_2$ 都是 $X$ 上的线性泛函

先验证 $f_1$ 为线性泛函：

$$
\begin{aligned}
f_1(\alpha x + \beta y) &= (\alpha x + \beta y)(0)\\
&= \alpha x(0) + \beta y(0)\\
&= \alpha f_1(x) + \beta f_1(y)
\end{aligned}
$$

再验证 $f_2$ 为线性泛函：

$$
\begin{aligned}
f_2(\alpha x + \beta y) &= \int_0^1 t(\alpha x(t) + \beta y(t)) dt\\
&= \alpha \int_0^1 tx(t) dt + \beta \int_0^1 ty(t) dt\\
&= \alpha f_2(x) + \beta f_2(y)
\end{aligned}
$$

### 2. $f_1 \notin X'$

假设 $f_1 \in X'$，则 $\exist M > 0, \forall x \in X, |f_1(x)| \le M \|x\|_1$。

取 $x_n(t) = \begin{cases} 1 - nt, & t \in [0, \frac{1}{n}]\\ 0, & t \in (\frac{1}{n}, 1] \end{cases}$，则 $\|x_n\|_1 = \int_0^1 |x_n(t)| dt = \int_0^{\frac{1}{n}} (1 - nt) dt = \frac{1}{2n} \to \infty$。

而 $f_1(x_n) = x_n(0) = 1$，与 $|f_1(x_n)| \le M \|x_n\|_1$ 矛盾，故 $f_1 \notin X'$。

### 3. $f_2 \in X'$，求出 $\|f_2\|$

$$
\begin{aligned}
|f_2(x)| &= \left| \int_0^1 tx(t) dt \right|\\
&\le \int_0^1 |t||x(t)| dt\\
&\le \int_0^1 |x(t)| dt\\
&= \|x\|_1
\end{aligned}
$$

故 $f_2 \in X'$ 且 $\|f_2\| \le 1$，下面求 $\|f_2\|$。

取 $x_n(t) = \begin{cases} 0, & t \in [0, \frac{n - 1}{n})\\ 2n^2t - 2n(n-1), & t \in [\frac{n - 1}{n}, 1]\end{cases}$，则 $\|x_n\|_1 = 1$。计算 $f_2(x_n)$：

$$
\begin{aligned}
f_2(x_n) &= \int_0^1 tx_n(t) dt\\
&= \int_{\frac{n - 1}{n}}^1 t(2n^2t - 2n(n-1)) dt\\
&= \int_{\frac{n - 1}{n}}^1 (2n^2t^2 - 2n(n-1)t) dt\\
&= \frac{2}{3} n^2 t^3 |_{{\frac{n - 1}{n}}}^1 - n(n-1)t^2 |_{{\frac{n - 1}{n}}}^1\\
&= 1 - \frac{1}{3n}
\end{aligned}
$$

故有 $\lim_{n \to \infty} f_2(x_n) = 1$，即 $\|f_2\| \ge 1$，故 $\|f_2\| = 1$。
